Wip for ack turing machine.

src/ack.lean
@@ -2,4 +2,76 @@ import computability.partrec
 import computability.partrec_code
 import computability.primrec
 import computability.tm_to_partrec
+import data.binnat
 
+def ack : ℕ → ℕ → ℕ 
+  | 0 n := n + 1
+  | (m+1) 0 := ack m 1
+  | (m+1) (n+1) := ack m (ack (m+1) n)
+
+def Γ : unit → Type := λ _, ℕ 
+
+open turing
+open turing.TM2
+open turing.TM2.stmt
+
+section util
+universes u₁ u₂ u₃ u₄
+
+notation `𝔹` := bool 
+notation `⋆` := unit.star
+
+def write_to_m : (ℕ × ℕ × 𝔹) → option ℕ → (ℕ × ℕ × 𝔹)
+  | ⟨m, n, _⟩ none := ⟨m, n, ff⟩
+  | ⟨m, n, b⟩ (some m') := ⟨m', n, b⟩
+
+def write_to_n : (ℕ × ℕ × 𝔹) → option ℕ → (ℕ × ℕ × 𝔹)
+  | ⟨m, n, _⟩ none := ⟨m, n, ff⟩
+  | ⟨m, n, b⟩ (some n') := ⟨m, n', b⟩
+
+abbreviation get_m (x : ℕ × ℕ × 𝔹) : Γ ⋆ := x.1 
+
+abbreviation get_has_failed (x : ℕ × ℕ × 𝔹) : 𝔹 := not x.2.2
+
+abbreviation get_is_m_zero (x : ℕ × ℕ × 𝔹) : 𝔹 := x.1 = 0
+abbreviation get_is_n_zero (x : ℕ × ℕ × 𝔹) : 𝔹 := x.2.1 = 0
+
+abbreviation get_succ_n (x : ℕ × ℕ × 𝔹) : Γ ⋆ := nat.succ x.2.1
+abbreviation get_pred_m (x : ℕ × ℕ × 𝔹) : Γ ⋆ := nat.pred x.1
+abbreviation get_pred_n (x : ℕ × ℕ × 𝔹) : Γ ⋆ := nat.pred x.2.1
+
+abbreviation recurse : TM2.stmt Γ unit (ℕ × ℕ × 𝔹) := load (λ _, (0,0, true)) $ goto (λ_, ⋆)
+abbreviation ack_tm_type := unit → turing.TM2.stmt Γ unit (ℕ × ℕ × 𝔹)
+abbreviation ack_cfg := TM2.cfg Γ unit (ℕ × ℕ × 𝔹)
+
+abbreviation mk_cfg (n m : ℕ) (l : list ℕ) : ack_cfg := TM2.cfg.mk (some ⋆) (n, m, tt) (λ _, m :: n :: l)
+
+def ack_tm : ack_tm_type
+  | _ :=
+    pop ⋆ write_to_m $
+      pop ⋆ write_to_n $
+        branch get_has_failed (push ⋆ get_m halt) $
+        branch get_is_m_zero (push ⋆ get_succ_n recurse) $
+          push ⋆ get_pred_m $
+            branch get_is_n_zero 
+              (push ⋆ (λ _, cast rfl (1:nat)) recurse)
+              (push ⋆ get_m $ push ⋆ get_pred_n recurse)
+
+example : ∀ x, nat.succ x ≠ 0 := nat.succ_ne_zero
+
+lemma registers_dont_matter_at_call_site (i n₁ n₂ m₁ m₂ : ℕ) (l : list ℕ) : 
+  TM2.step ack_tm (mk_cfg n₁ m₁ (i :: l)) = TM2.step ack_tm (mk_cfg n₂ m₂ (i :: l)) := 
+  begin
+    cases l; simp; unfold ack_tm; simp;
+    unfold write_to_m write_to_n; simp;
+    cases m₂; cases m₁,
+    case nat.zero nat.zero {
+      
+    },
+  end
+
+lemma ack_tm_correct_aux (nₜ mₜ n₁ m₁: ℕ) (l : list ℕ) : ∃ n₂ m₂ : ℕ, turing.TM2.reaches ack_tm (TM2.cfg.mk (some ⋆) (n₁, m₁, tt) ( λ _, mₜ :: nₜ :: l) : ack_cfg) ((TM2.cfg.mk (some ⋆) (n₁, m₁, tt) ( λ _, mₜ :: nₜ :: l) : ack_cfg))
+
+theorem ack_tm_correct (m n : ℕ) : TM2.eval ack_tm ⋆ [n, m] = (pure ∘ pure) (ack m n) :=
+  begin
+  end
